verification to agile

code/ecdsap256sha2/Hacl.Impl.ECDSA.P256SHA256.Verification.fst
@@ -33,6 +33,9 @@ open Lib.ByteSequence
 open Lib.IntVector.Intrinsics
 
 
+open Spec.Hash.Definitions
+open Hacl.Hash.Definitions
+
 open FStar.Mul
 
 module H = Spec.Agile.Hash
@@ -93,28 +96,49 @@ let ecdsa_verification_step1 r s =
   isRCorrect && isSCorrect
 
 
-inline_for_extraction noextract
-val ecdsa_verification_step23: hashAsFelem : felem -> mLen: size_t -> m: lbuffer uint8 mLen -> Stack unit
-  (requires fun h -> live h hashAsFelem /\ live h m)
-  (ensures  fun h0 _ h1 -> modifies (loc hashAsFelem) h0 h1 /\
-  (
+val ecdsa_verification_step23: alg: hash_alg {SHA2_256? alg \/ SHA2_384? alg \/ SHA2_512? alg (* and blake one day *)}
+  ->  mLen: size_t -> m: lbuffer uint8 mLen -> result: felem -> Stack unit
+  (requires fun h -> live h m /\ live h result )
+  (ensures fun h0 _ h1 -> modifies (loc result) h0 h1 /\
+    (
       assert_norm (pow2 32 < pow2 61);
-      let hashM = H.hash Def.SHA2_256 (as_seq h0 m) in 
-      as_nat h1 hashAsFelem == nat_from_bytes_be hashM % prime_p256_order)
+      assert_norm (pow2 32 < pow2 125);
+      let hashM = (hashSpec alg) (as_seq h0 m) in 
+      let cutHashM = Lib.Sequence.sub hashM 0 32 in 
+      as_nat h1 result = nat_from_bytes_be cutHashM % prime_p256_order
+    )
   )
 
-let ecdsa_verification_step23 hashAsFelem mLen m =
-  push_frame();
-        assert_norm (pow2 32 < pow2 61);
-  let h0 = ST.get() in
-  let mHash = create (size 32) (u8 0) in
-  hash_256 m mLen mHash;
-  toUint64ChangeEndian mHash hashAsFelem;
-  let h1 = ST.get() in
-  lemma_core_0 hashAsFelem h1;
-  reduction_prime_2prime_order hashAsFelem hashAsFelem;
-  Spec.ECDSA.changeEndianLemma (uints_from_bytes_be #U64 #_ #4 (as_seq h1 mHash));
-  uints_from_bytes_be_nat_lemma #U64 #_ #4 (as_seq h1 mHash);
+
+let ecdsa_verification_step23 alg mLen m result = 
+  assert_norm (pow2 32 < pow2 61);
+  assert_norm (pow2 32 < pow2 125);
+  push_frame(); 
+    let h0 = ST.get() in 
+  let sz: FStar.UInt32.t = hash_len alg in
+  let mHash = create sz (u8 0) in    
+  
+  begin
+  match alg with 
+    |SHA2_256 ->
+      hash_256 m mLen mHash
+    |SHA2_384 ->
+      hash_384 m mLen mHash
+    |SHA2_512 -> 
+      hash_512 m mLen mHash
+  end;
+  
+  let cutHash = sub mHash (size 0) (size 32) in 
+  toUint64ChangeEndian cutHash result;
+  
+  let h1 = ST.get() in 
+ 
+  reduction_prime_2prime_order result result;
+
+  lemma_core_0 result h1;
+  Spec.ECDSA.changeEndianLemma (uints_from_bytes_be #U64 #_ #4 (as_seq h1 cutHash));
+  uints_from_bytes_be_nat_lemma #U64 #_ #4 (as_seq h1 cutHash);
+
   pop_frame()
 
 
@@ -365,7 +389,8 @@ let compare_felem_bool a b   =
 
 
 val ecdsa_verification_core:
-    publicKeyPoint:point
+  alg: hash_alg {SHA2_256? alg \/ SHA2_384? alg \/ SHA2_512? alg}
+  -> publicKeyPoint:point
   -> hashAsFelem:felem
   -> r:lbuffer uint64 (size 4)
   -> s:lbuffer uint64 (size 4)
@@ -398,8 +423,11 @@ val ecdsa_verification_core:
       modifies (loc publicKeyPoint |+| loc hashAsFelem |+| loc xBuffer |+| loc tempBuffer) h0 h1 /\
        (
          assert_norm (pow2 32 < pow2 61);
-	 let hashM = H.hash Def.SHA2_256 (as_seq h0 m) in 
-	 let hashNat = nat_from_bytes_be hashM % prime_p256_order in 
+	 assert_norm (pow2 32 < pow2 125);
+	 
+	 let hashM = (hashSpec alg) (as_seq h0 m) in 
+	 let cutHashM = Lib.Sequence.sub hashM 0 32 in 
+	 let hashNat =  nat_from_bytes_be cutHashM % prime_p256_order in 
 	 
          let p0 = pow (as_nat h0 s) (prime_p256_order - 2) * hashNat % prime_p256_order in 
 	 let p1 = pow (as_nat h0 s) (prime_p256_order - 2) * as_nat h0 r % prime_p256_order in 
@@ -416,13 +444,14 @@ val ecdsa_verification_core:
       )
   )
 
-let ecdsa_verification_core publicKeyBuffer hashAsFelem r s mLen m xBuffer tempBuffer =
+let ecdsa_verification_core alg publicKeyBuffer hashAsFelem r s mLen m xBuffer tempBuffer =
   assert_norm (pow2 32 < pow2 61 - 1);
+  assert_norm (pow2 32 < pow2 125);
   push_frame();
   let tempBufferU8 = create (size 64) (u8 0) in
   let bufferU1 = sub tempBufferU8 (size 0) (size 32) in
   let bufferU2 = sub tempBufferU8 (size 32) (size 32) in
-  ecdsa_verification_step23 hashAsFelem mLen m;
+  ecdsa_verification_step23 alg mLen m hashAsFelem;
   ecdsa_verification_step4  bufferU1 bufferU2 r s hashAsFelem;
   let r = ecdsa_verification_step5 xBuffer publicKeyBuffer bufferU1 bufferU2 tempBuffer in
   pop_frame();
@@ -431,7 +460,8 @@ let ecdsa_verification_core publicKeyBuffer hashAsFelem r s mLen m xBuffer tempB
 
 (* This code is not side channel resistant *)
 val ecdsa_verification_:
-    pubKey:lbuffer uint64 (size 8)
+  alg: hash_alg {SHA2_256? alg \/ SHA2_384? alg \/ SHA2_512? alg}
+  -> pubKey:lbuffer uint64 (size 8)
   -> r:lbuffer uint64 (size 4)
   -> s: lbuffer uint64 (size 4)
   -> mLen: size_t
@@ -440,15 +470,18 @@ val ecdsa_verification_:
     (requires fun h -> live h pubKey /\ live h r /\ live h s /\ live h m)
     (ensures fun h0 result h1 ->
       assert_norm (pow2 32 < pow2 61);
+      assert_norm (pow2 32 < pow2 125);
       let pubKeyX = as_nat h0 (gsub pubKey (size 0) (size 4)) in
       let pubKeyY = as_nat h0 (gsub pubKey (size 4) (size 4)) in
       let r = as_nat h0 r in
       let s = as_nat h0 s in
       modifies0 h0 h1 /\
-      result == Spec.ECDSA.ecdsa_verification (pubKeyX, pubKeyY) r s (v mLen) (as_seq h0 m))
+      result == Spec.ECDSA.ecdsa_verification alg (pubKeyX, pubKeyY) r s (v mLen) (as_seq h0 m))
 
-let ecdsa_verification_ pubKey r s mLen m =
+
+let ecdsa_verification_ alg pubKey r s mLen m =
   assert_norm (pow2 32 < pow2 61);
+  assert_norm (pow2 32 < pow2 125);
   push_frame();
   let tempBufferU64 = create (size 120) (u64 0) in
   let publicKeyBuffer = sub tempBufferU64 (size 0) (size 12) in
@@ -471,7 +504,7 @@ let ecdsa_verification_ pubKey r s mLen m =
       false
       end
     else
-      let state = ecdsa_verification_core publicKeyBuffer hashAsFelem r s mLen m xBuffer tempBuffer in
+      let state = ecdsa_verification_core alg publicKeyBuffer hashAsFelem r s mLen m xBuffer tempBuffer in
       if state = false then
         begin
         pop_frame();
@@ -486,7 +519,8 @@ let ecdsa_verification_ pubKey r s mLen m =
 
 
 val ecdsa_verification:
-    pubKey:lbuffer uint8 (size 64)
+  alg: hash_alg {SHA2_256? alg \/ SHA2_384? alg \/ SHA2_512? alg}
+  -> pubKey:lbuffer uint8 (size 64)
   -> r:lbuffer uint8 (size 32)
   -> s:lbuffer uint8 (size 32)
   -> mLen:size_t
@@ -495,15 +529,17 @@ val ecdsa_verification:
     (requires fun h -> live h pubKey /\ live h r /\ live h s /\ live h m)
     (ensures fun h0 result h1 ->
       assert_norm (pow2 32 < pow2 61);
+      assert_norm (pow2 32 < pow2 125);
       let publicKeyX = nat_from_bytes_be (as_seq h1 (gsub pubKey (size 0) (size 32))) in
       let publicKeyY = nat_from_bytes_be (as_seq h1 (gsub pubKey (size 32) (size 32))) in
       let r = nat_from_bytes_be (as_seq h1 r) in
       let s = nat_from_bytes_be (as_seq h1 s) in
       modifies0 h0 h1 /\
-      result == Spec.ECDSA.ecdsa_verification (publicKeyX, publicKeyY) r s (v mLen) (as_seq h0 m))
+      result == Spec.ECDSA.ecdsa_verification alg (publicKeyX, publicKeyY) r s (v mLen) (as_seq h0 m))
 
-let ecdsa_verification pubKey r s mLen m =
+let ecdsa_verification alg pubKey r s mLen m =
   assert_norm (pow2 32 < pow2 61);
+  assert_norm (pow2 32 < pow2 125);
   push_frame();
   let h0 = ST.get() in 
     let publicKeyAsFelem = create (size 8) (u64 0) in
@@ -531,7 +567,7 @@ let ecdsa_verification pubKey r s mLen m =
       lemma_core_0 sAsFelem h1;
       uints_from_bytes_le_nat_lemma #U64 #SEC #4 (as_seq h1 s);
 
-    let result = ecdsa_verification_ publicKeyAsFelem rAsFelem sAsFelem mLen m in 
+    let result = ecdsa_verification_ alg publicKeyAsFelem rAsFelem sAsFelem mLen m in 
     pop_frame();
 
     changeEndianLemma (uints_from_bytes_be (as_seq h1 (gsub pubKey (size 0) (size 32))));
